examples/TrivialADTCache.v
@@ -1,6 +1,6 @@
 Require Import QueryStructureNotations.
 Require Import ListImplementation.
-Require Import AddCache ADTCache CacheADT.
+Require Import ComputationalADT AddCache ADTCache CacheADT.
 
 Definition MySchema :=
   Query Structure Schema
@@ -46,50 +46,23 @@ Definition MySpec : ADT MySig :=
 
 Section CachingRefinement.
 
-  Require Import ComputationalADT.
-
   Definition CacheSpec := @CacheSpec string nat.
-  Variable LRUCache : FullySharpened CacheSpec.
+  Variable LRUCache : Sharpened CacheSpec.
   Definition PopCache := projT1 LRUCache.
   Definition PopCacheAbs : Rep CacheSpec -> Rep PopCache -> Prop :=
-    AbsR (fst (projT2 LRUCache)).
-  Definition PopCacheComp := snd (projT2 LRUCache).
+    AbsR (projT2 LRUCache).
+  (* Definition PopCacheComp := snd (projT2 LRUCache). *)
 
-  Definition CallMethod'
-             (Sig : ADTSig)
-             (A : ADT Sig)
-             (CompA : is_computationalADT A)
-             (idx : MethodIndex Sig)
-             (r : Rep A)
-             (i : fst (MethodDomCod Sig idx))
-             : Rep A * snd (MethodDomCod Sig idx) :=
-    is_computational_val (proj2 CompA idx r i).
-
-  Notation CallMethod CompADT idx r i :=
-    (CallMethod' CompADT {|bindex := idx |} r i).
-
-  Definition CallConstructor'
-             (Sig : ADTSig)
-             (A : ADT Sig)
-             (CompA : is_computationalADT A)
-             (idx : ConstructorIndex Sig)
-             (i : ConstructorDom Sig idx)
-             : Rep A :=
-    is_computational_val (proj1 CompA idx i).
-
-  Notation CallConstructor CompADT idx i :=
-    (CallConstructor' CompADT {|bindex := idx |} i).
-
-  Definition EmptyCache := CallConstructor PopCacheComp "EmptyCache" ().
+  (* Definition EmptyCache := CallConstructor PopCacheComp "EmptyCache" ().
   Definition InsertKey r i := CallMethod PopCacheComp "AddKey" r i.
   Definition LookupKey r i := CallMethod PopCacheComp "LookupKey" r i.
-  Definition UpdateKey r i := CallMethod PopCacheComp "UpdateKey" r i.
+  Definition UpdateKey r i := CallMethod PopCacheComp "UpdateKey" r i. *)
 
   Definition BreedCacheSpec
              (or : UnConstrQueryStructure MySchema)
              (cache : Rep CacheSpec) :=
-    forall breed r pop,
-      r (breed,  pop)
+    forall breed pop,
+      cache (breed,  pop)
       -> refine
            (Count (For (UnConstrQuery_In or ``("Dog")
                                          (fun d =>
@@ -104,30 +77,13 @@ Section CachingRefinement.
      (origRep or) ! "Dog" ≃ snd (fst nr)) /\
     PopCacheAbs (cachedVal or) (snd nr).
 
-  Lemma refine_Pick_Some {A B}
-  : forall (P : Ensemble B) (c e : Comp A) (t : B -> Comp A),
-      (forall b, P b -> refine c (t b))
-      -> ((forall b, ~ P b) -> refine c e)
-      -> refine c
-                (b <- {b | forall b',
-                             (b = Some b' -> P b')
-                             /\ (b = None -> forall b', ~ P b')};
-                 match b with
-                   | Some b => t b
-                   | None => e
-                 end).
-  Proof.
-    unfold refine; intros; apply computes_to_inv in H1; destruct_ex; intuition.
-    destruct x; inversion_by computes_to_inv; eauto.
-  Qed.
-
   Definition My :
     Sharpened MySpec.
   Proof.
     unfold MySpec.
-    
+
     start honing QueryStructure.
-    
+
     hone representation using (cachedRep_AbsR BreedCacheSpec).
 
     hone method "YoungOwners'Breeds".
@@ -140,241 +96,293 @@ Section CachingRefinement.
 
     hone method "BreedPopulation".
     { simplify with monad laws.
-      apply refine_Pick_Some with (P := fun v => cachedVal r_n (n, v)); intros.
-      { refine pick val _.
-        simplify with monad laws; cbv beta; simpl.
-        destruct H0; subst.
-        unfold BreedCacheSpec in *.
-        apply H2 in H1.
+      etransitivity.
+      apply refine_Pick_If_Then_Opt with (P := fun v => cachedVal r_n (n, v)); intros.
+      { destruct H0; subst; unfold BreedCacheSpec in *|- .
         subst_strings.
+        apply H2 in H1.
         rewrite H1.
+        simplify with monad laws; cbv beta; simpl.
+        refine pick val _; try split; eauto.
         simplify with monad laws.
         finish honing.
       }
       {
         unfold cachedRep_AbsR in *|-; simpl; split_and; subst.
-        rewrite refine_under_bind'; [reflexivity | ].
+        rewrite refine_under_bind; [reflexivity | ].
         intros; rewrite refine_pick_cachedRep.
         simplify with monad laws.
-        intros; pose (callMeth CacheSpec "AddKey" (cachedVal r_n) (n, x)); simpl in c.
-        
-        rewrite refine_pick_val with 
-                (A := (Ensemble (string * nat)))
-                (a := callMeth CacheSpec "AddKey" (cachedVal r_n) (n, x)).
-
-                         cachedVal := c |}).
-
-        intros; rewrite refineEquiv_pick_pair.
-        intros; pose (callMeth CacheSpec "AddKey" (cachedVal r_n) (n, x)).
-        re
-
-        simpl in c.
-        intros; rewrite refine_pick_val with 
-                (A := cachedRep (UnConstrQueryStructure MySchema) (Ensemble (string * nat)))
-                (a := {| origRep := origRep r_n; 
-                         cachedVal := c |}).
+        assert (refine {cv | BreedCacheSpec (origRep r_n) cv}
+                       (c <- (callMeth CacheSpec "AddKey" (cachedVal r_n) (n, a));
+                        ret (fst c))).
+        repeat econstructor.
+        inversion_by computes_to_inv; subst.
+        unfold BreedCacheSpec; intros.
+        unfold SubEnsembleInsert in H1.
+        intros H7; pose proof (H1 _ H3).
+        destruct H4; injections.
+        unfold refine; intros; inversion_by computes_to_inv; subst; eauto.
+        apply H2; eauto.
+        rewrite H1.
         simplify with monad laws.
-
         finish honing.
-        cbv beta. simpl.
-        refine pick val ({| origRep := rep r_n; cachedVal := callMeth CacheSpec "insert" r_n (n, b) |}).
-        rewrite refine_pick_val 
-        unfold cachedRep_AbsR in H0; intuition; subst.
-    eapply refine_if with (b := if (string_dec n "Dachshund")
-                                then true
-                                else false).
-    { find_if_inside; try congruence; subst.
-      intros; unfold BreedCacheSpec in H2.
-      subst_body.
-      setoid_rewrite H2; simplify with monad laws; simpl.
-      reflexivity. }
-    { find_if_inside; try congruence; subst.
-      simpl; reflexivity.
+      }
+      finish honing.
     }
-  }
 
-  hone constructor "Empty".
-  { simplify with monad laws.
-    rewrite refine_pick_cachedRep.
-    rewrite refine_pick_val with (A := nat)
-                                   (a := 0).
-    simplify with monad laws; finish honing.
-    unfold BreedCacheSpec; simpl.
-    unfold pointwise_relation; intros; setoid_rewrite refine_Count.
-    setoid_rewrite refine_For_In_Empty.
-    simplify with monad laws; reflexivity.
-  }
+    hone constructor "Empty".
+    { simplify with monad laws.
+      rewrite refine_pick_cachedRep.
+      refine pick val (fun _ : string * nat => False).
+      simplify with monad laws; finish honing.
+      unfold BreedCacheSpec; simpl.
+      intuition.
+    }
 
-  hone method "AddDog".
-  {
-    simplify with monad laws; cbv beta; simpl.
-    etransitivity.
-    eapply refine_bind_pick; intros.
-    rewrite refine_pick_cachedRep.
-    simplify with monad laws.
-    unfold BreedCacheSpec; simpl.
-    pose_string_ids.
-
-    rewrite refine_pick_val.
-    simplify with monad laws; higher_order_1_reflexivity.
-    unfold pointwise_relation; intros.
-    intros; etransitivity.
-    apply refine_refine_Count.
-    apply refine_For_In_Insert.
-    unfold In, not; intros; eapply H1;
-    [ eapply H2
-     | subst_body; auto ].
-    rewrite refine_Count_bind_bind_app.
-    unfold cachedRep_AbsR, BreedCacheSpec in H0; split_and; subst.
-    pose_string_ids.
-    setoid_rewrite H3.
-    simplify with monad laws.
-    subst_body.
-    etransitivity.
-    pose (n!"Breed"); simpl in *.
-    eapply refine_if with (b := if (string_dec d "Dachshund")
-                                then true
-                                else false);
-    find_if_inside; try congruence; intros.
-    subst_body.
-    rewrite refine_Count; simplify with monad laws.
-    unfold Query_Where, Query_Return.
-    rewrite refine_pick_val.
-    simplify with monad laws; reflexivity.
-    intuition.
-    rewrite refine_Count; simplify with monad laws.
-    unfold Query_Where, Query_Return.
-    rewrite refine_pick_val.
-    simplify with monad laws; reflexivity.
-    intuition.
-    eapply refineEquiv_if_ret.
-    simpl.
-    unfold cachedRep_AbsR in H0; intuition.
-    subst.
-    finish honing.
-  }
-
-  hone representation using MyListImpl_abs.
-  hone constructor "Empty".
-  { simplify with monad laws.
-    unfold MyListImpl_abs, GetUnConstrRelation; simpl.
-    rewrite refineEquiv_pick_pair_pair.
-    rewrite refine_pick_val by
-        apply EnsembleIndexedListEquivalence_Empty;
-    simplify with monad laws.
-    rewrite refine_pick_val by
-        apply EnsembleIndexedListEquivalence_Empty;
+    hone method "AddDog".
+    {
+      simplify with monad laws; cbv beta; simpl.
+      etransitivity.
+      eapply refine_bind_pick; intros.
+      rewrite refine_pick_cachedRep.
       simplify with monad laws.
-    rewrite refineEquiv_pick_eq';
+      assert (refine {cv |
+                      BreedCacheSpec
+                        (UpdateUnConstrRelation or ``(StringId7)
+                                                (InsertQSSpecs.EnsembleInsert
+                                                   {| tupleIndex := a; indexedTuple := n |}
+                                                   (or!StringId7)%QueryImpl)) cv}
+                     (r' <- callMeth CacheSpec "UpdateKey" (cachedVal r_n) (n!"Breed", S);
+                      ret (fst r'))).
+      repeat econstructor.
+      inversion_by computes_to_inv; subst.
+      unfold BreedCacheSpec; intros.
+      simpl; pose_string_ids.
+      etransitivity.
+      apply refine_refine_Count.
+      apply refine_For_In_Insert.
+      unfold In, not; intros; eapply H1;
+      [ eapply H4
+      | subst_body; auto ].
+      rewrite refine_Count_bind_bind_app.
+      unfold cachedRep_AbsR, BreedCacheSpec in H0; split_and; subst.
+      pose_string_ids.
+      pose (n!"Breed"); simpl in *.
+      etransitivity.
+      apply refine_if with (b := if (string_dec d breed)
+                                 then true
+                                 else false);
+        find_if_inside; try discriminate; subst; intros.
+      { setoid_rewrite refine_Count at 1; simplify with monad laws;
+        unfold Query_Where; refine pick val [()];
+        [ | intuition; econstructor].
+        simplify with monad laws.
+        apply H2 in H3; unfold In in *.
+        subst_strings.
+        destruct H3; split_and.
+        destruct_ex; split_and; subst.
+        rewrite (H6 _ _ H8).
+        simplify with monad laws; simpl; reflexivity.
+        unfold EnsembleRemove in H3; simpl in H3; elimtype False; eapply H3;
+        reflexivity.
+      }
+      {
+        setoid_rewrite refine_Count at 1; simplify with monad laws;
+        unfold Query_Where; refine pick val [];
+        [ | intuition; econstructor].
+        simplify with monad laws.
+        apply H2 in H3; unfold In in *.
+        subst_strings.
+        destruct H3; split_and; try congruence.
+        destruct H3; rewrite (H6 _ _ H4); reflexivity.
+      }
+      find_if_inside; reflexivity.
+      subst_strings; setoid_rewrite H2.
       simplify with monad laws.
-    finish honing.
-  }
+      higher_order_1_reflexivity.
+      cbv beta.
+      unfold cachedRep_AbsR in H0; intuition.
+      subst.
+      finish honing.
+    }
 
-  hone method "YoungOwners'Breeds".
-  {
-    simplify with monad laws; simpl.
-    unfold MyListImpl_abs in *; intuition.
-    rewrite refine_List_Query_In by apply H3.
-    rewrite refine_Join_List_Query_In by apply H0.
-    rewrite refine_List_Query_In_Where.
-    rewrite refine_List_Query_In_Where.
-    rewrite refine_List_For_Query_In_Return;
+    hone representation using MyListImpl_abs.
+    hone constructor "Empty".
+    { simplify with monad laws.
+      unfold MyListImpl_abs, GetUnConstrRelation; simpl.
+      rewrite refineEquiv_pick_pair_pair.
+      rewrite refine_pick_val by
+          apply EnsembleIndexedListEquivalence_Empty;
+        simplify with monad laws.
+      rewrite refine_pick_val by
+          apply EnsembleIndexedListEquivalence_Empty;
+        simplify with monad laws.
+      (* Rewriting with the cache implementation. *)
+      assert (refine {c | PopCacheAbs (fun _ : string * nat => False) c}
+                     (callCons PopCache "EmptyCache" ())).
+      {
+        pose (ADTRefinementPreservesConstructors (projT2 LRUCache) {| bindex := "EmptyCache" |}).
+        simpl in r; rewrite <- r.
+        rewrite refineEquiv_bind_unit; f_equiv.
+      }
+      rewrite H0.
+      finish honing.
+    }
+
+    hone method "YoungOwners'Breeds".
+    {
+      pose_string_ids.
       simplify with monad laws; simpl.
-
-    setoid_rewrite refineEquiv_pick_pair_pair.
-    setoid_rewrite refineEquiv_pick_eq'.
-    simplify with monad laws.
-    simpl in *.
-    rewrite refine_pick_val by eassumption.
-    simplify with monad laws.
-    rewrite refine_pick_val by eassumption.
-    simplify with monad laws.
-    rewrite H2.
-    finish honing.
-  }
-
-  hone method "BreedPopulation".
-  {
-    eapply refine_if with (b := if (string_dec n "Dachshund")
-                                then true
-                                else false);
-    find_if_inside; try congruence; intros;
-    simplify with monad laws; simpl.
-
-    {
       unfold MyListImpl_abs in *; intuition.
-      setoid_rewrite refineEquiv_pick_pair_pair.
-      setoid_rewrite refineEquiv_pick_eq'.
-      simplify with monad laws.
-      rewrite refine_pick_val by eassumption.
-      simplify with monad laws.
-      rewrite refine_pick_val by eassumption.
-      simplify with monad laws.
-      rewrite H3.
-      reflexivity.
-    }
-
-    {
-      unfold MyListImpl_abs in *; split_and.
-      rewrite refine_Count; simplify with monad laws.
-      rewrite refine_List_Query_In by eassumption.
-      simpl; subst_body.
-      setoid_rewrite refine_List_Query_In_Where.
+      rewrite refine_List_Query_In by apply H3.
+      subst_strings.
+      rewrite refine_Join_List_Query_In by apply H0.
+      pose_string_ids.
+      rewrite refine_List_Query_In_Where.
+      rewrite refine_List_Query_In_Where.
       rewrite refine_List_For_Query_In_Return;
         simplify with monad laws; simpl.
-      setoid_rewrite refineEquiv_pick_pair_pair.
-      setoid_rewrite refineEquiv_pick_eq'.
+      refine pick pair; simplify with monad laws;
+      refine pick pair; simplify with monad laws.
+      simpl in *.
+      refine pick val _ ; try eassumption.
       simplify with monad laws.
-      rewrite refine_pick_val by eassumption.
+      refine pick val _ ; try eassumption.
       simplify with monad laws.
-      rewrite refine_pick_val by eassumption.
+      refine pick val _ ; try eassumption.
       simplify with monad laws.
-      rewrite H3.
-      reflexivity.
-    }
+      finish honing.
     }
 
-  hone method "AddDog".
-  {
-    unfold MyListImpl_abs in *; split_and.
-    simplify with monad laws; simpl.
-    rewrite refine_pick_val with (A := nat) (a := length (snd (fst r_n))).
-    simplify with monad laws; simpl.
-    pose_string_ids.
-    setoid_rewrite refineEquiv_pick_pair_pair; simpl.
-    setoid_rewrite refineEquiv_pick_eq'.
-    simplify with monad laws.
-    subst_strings.
-      match goal with
-          |- context
-               [{a | EnsembleIndexedListEquivalence
-                       ((@UpdateUnConstrRelation ?QSSchema ?c ?Ridx
-                                                (EnsembleInsert ?n (?c!?R)))!?R')%QueryImpl a}%comp] =>
-          let H := fresh in
-          generalize ((@ImplementListInsert_neq QSSchema
-                                                {| bindex := R' |}
-                                                {| bindex := R |} n c)) as H; intros; setoid_rewrite H
-      end; try reflexivity; try eassumption.
+    hone method "BreedPopulation".
+    { simplify with monad laws.
+      pose (callMeth PopCache "LookupKey" (snd r_n) n).
+      assert (refine {b | forall b' : nat, b = Some b' -> cachedVal or (n, b')}
+                     (o <- callMeth PopCache "LookupKey" (snd r_n) n;
+                      ret (snd o))).
+      {
+        pose (ADTRefinementPreservesMethods (projT2 LRUCache) {| bindex := "LookupKey" |}
+                                            (cachedVal or) (snd r_n) n (proj2 H0)).
+        simpl in r.
+        subst_strings.
+        rewrite <- r.
+        unfold refine; intros; inversion_by computes_to_inv; subst.
+        simpl in *.
+        econstructor; intros; eapply H2; eauto.
+      }
+      subst_strings; setoid_rewrite H1; simplify with monad laws.
+      etransitivity; [apply refine_under_bind | ]; intros.
+      rewrite refine_If_Opt_Then_Else_Bind; apply refine_If_Opt_Then_Else.
+      { unfold pointwise_relation; intros.
+        simplify with monad laws.
+        refine pick val _; simpl; eauto.
+        simplify with monad laws; higher_order_1_reflexivity.
+      }
+      {
+        unfold MyListImpl_abs in *; split_and.
+        rewrite refine_Count; simplify with monad laws.
+        rewrite refine_List_Query_In by eassumption.
+        simpl; subst_body.
+        setoid_rewrite refine_List_Query_In_Where.
+        rewrite refine_List_For_Query_In_Return;
+          simplify with monad laws.
+        etransitivity.
+        apply refine_bind; [reflexivity | unfold pointwise_relation; intros].
+        refine pick pair; simplify with monad laws.
+        refine pick pair; simplify with monad laws.
+        rewrite refine_pick_val by eassumption.
+        simplify with monad laws.
+        rewrite refine_pick_val by eassumption.
+        simplify with monad laws.
+        higher_order_1_reflexivity.
+        pose (callMeth PopCache "AddKey" (snd r_n)).
+        assert (forall kv, refine
+                             (or <- (callMeth CacheSpec "AddKey" (cachedVal or) kv);
+                              {b | PopCacheAbs (fst or) b})
+                             (nr <- c kv; ret (fst nr))).
+        {
+          intros;
+          pose (ADTRefinementPreservesMethods (projT2 LRUCache) {| bindex := "AddKey" |}
+                                              _ _ kv H4).
+          unfold c; subst_strings. rewrite <- r.
+          repeat rewrite refineEquiv_bind_bind.
+          f_equiv; unfold pointwise_relation; intros.
+          rewrite refineEquiv_bind_bind; simpl.
+          setoid_rewrite refineEquiv_bind_unit; simpl.
+          setoid_rewrite refineEquiv_unit_bind.
+          reflexivity.
+        }
+        simpl in H.
+        rewrite <- refineEquiv_bind_bind.
+        rewrite H; simplify with monad laws.
+        reflexivity.
+      }
+      finish honing.
+    }
+
+    hone method "AddDog".
+    {
+      unfold MyListImpl_abs in *; split_and.
+      pose_string_ids.
+      simplify with monad laws; simpl.
+      rewrite refine_pick_val with (A := nat) (a := length (snd (fst r_n))).
+      simplify with monad laws; simpl.
+      pose_string_ids.
+      etransitivity.
+      apply refine_bind; [reflexivity | unfold pointwise_relation; intros].
+      refine pick pair; simplify with monad laws.
+      refine pick pair; simplify with monad laws.
+      rewrite refine_pick_val by eassumption.
       simplify with monad laws.
+      subst_strings.
       match goal with
           |- context
                [{a | EnsembleIndexedListEquivalence
                        ((@UpdateUnConstrRelation ?QSSchema ?c ?Ridx
-                                                (EnsembleInsert ?n (?c!?R)))!?R)%QueryImpl a}%comp] =>
+                                                 (InsertQSSpecs.EnsembleInsert ?n (?c!?R)))!?R)%QueryImpl a}%comp] =>
           let H := fresh in
           generalize ((@ImplementListInsert_eq QSSchema
-                                                {| bindex := R |}
-                                                n c)) as H; intros; setoid_rewrite H
+                                               {| bindex := R |}
+                                               n c)) as H; intros; setoid_rewrite H
       end; try reflexivity; try eassumption.
       simplify with monad laws.
-      rewrite H2.
+      higher_order_1_reflexivity.
+      pose (callMeth PopCache "UpdateKey" (snd r_n)).
+      assert (forall kv, refine
+                           (or <- (callMeth CacheSpec "UpdateKey" (cachedVal or) kv);
+                            {b | PopCacheAbs (fst or) b})
+                           (nr <- c kv; ret (fst nr))).
+      {
+        intros;
+        pose (ADTRefinementPreservesMethods (projT2 LRUCache) {| bindex := "UpdateKey" |}
+                                            _ _ kv H2).
+        unfold c; subst_strings. rewrite <- r.
+        repeat rewrite refineEquiv_bind_bind.
+        f_equiv; unfold pointwise_relation; intros.
+        rewrite refineEquiv_bind_bind; simpl.
+        setoid_rewrite refineEquiv_bind_unit; simpl.
+        setoid_rewrite refineEquiv_unit_bind.
+        reflexivity.
+      }
+      simpl in H1.
+      rewrite <- refineEquiv_bind_bind.
+      subst_strings.
+      set (n!"Breed").
+      specialize (H1 (d, S )).
+      subst_body.
+      rewrite H1.
+      simplify with monad laws.
       finish honing.
-      congruence.
       intros; destruct H3 as [H3 _].
       intros; eapply lt_irrefl.
       setoid_rewrite <- H4 in H3; eapply H3.
       eauto.
-  }
+    }
 
-  finish sharpening.
-Defined.
+    finish sharpening.
+
+  Defined.
+
+End CachingRefinement.
+
+Check (My (BoundedStringCacheADT nat 29)).
