src/ADT/ComputationalADT.v
@@ -40,3 +40,22 @@ Definition is_computationalADT (Sig : ADTSig) (A : ADT Sig) :=
      is_computational (Constructors A idx i))
   /\ (forall (idx : MethodIndex Sig) i r,
         is_computational (Methods A idx i r)).
+
+  Definition CallComputationalMethod
+             (Sig : ADTSig)
+             (A : ADT Sig)
+             (CompA : is_computationalADT A)
+             (idx : MethodIndex Sig)
+             (r : Rep A)
+             (i : fst (MethodDomCod Sig idx))
+             : Rep A * snd (MethodDomCod Sig idx) :=
+    is_computational_val (proj2 CompA idx r i).
+
+  Definition CallComputationalConstructor
+             (Sig : ADTSig)
+             (A : ADT Sig)
+             (CompA : is_computationalADT A)
+             (idx : ConstructorIndex Sig)
+             (i : ConstructorDom Sig idx)
+             : Rep A :=
+    is_computational_val (proj1 CompA idx i).
